Basic exercises finished

SimplyTypedLambdaCalculus.v.d
@@ -1,2 +1,0 @@
-SimplyTypedLambdaCalculus.vo SimplyTypedLambdaCalculus.glob SimplyTypedLambdaCalculus.v.beautified: SimplyTypedLambdaCalculus.v ./Maps.vo
-SimplyTypedLambdaCalculus.vio: SimplyTypedLambdaCalculus.v ./Maps.vio
