SimplyTypedLambdaCalculus.v
@@ -64,36 +64,49 @@ reflexivity.
 Qed.
 
 Fixpoint beq_type (A:type) (B:type) :=
-  match A with
-  | tvar a   => match B with
-                | tvar b => beq_string a b
-                | _      => false
-                end
-  | tarr C D => match B with
-                | tarr E F => (beq_type C E) 
-                              && (beq_type E F)
-                | _        => false
-                end
-  end.
+  match A, B with
+  | tvar a, tvar b =>
+      beq_string a b
+  | tarr A1 A2, tarr B1 B2 =>
+      beq_type A1 B1 && beq_type A2 B2
+  | _,_ =>
+      false
+end.
+
+Lemma beq_type_eq : forall A B,
+beq_type A B = true -> A = B.
+Proof.
+intros A.
+induction A; intros B Hbeq; 
+destruct B; inversion Hbeq.
+- apply beq_string_true_iff in Hbeq. 
+  rewrite Hbeq. reflexivity.
+- apply andb_prop in H0. 
+  destruct H0 as [Hbeq1 Hbeq2].
+  apply IHA1 in Hbeq1.
+  apply IHA2 in Hbeq2.
+  rewrite Hbeq1. rewrite Hbeq2.
+  reflexivity.
+Qed.
+
+Lemma beq_type_refl : forall (A: type),
+beq_type A A = true.
+Proof.
+induction A.
++ simpl. rewrite <- beq_string_refl. reflexivity.
++ simpl. rewrite IHA1. rewrite IHA2. reflexivity.
+Qed.
 
 Fixpoint beq_term (M: term) (N: term) :=
-  match M with
-  | var m => match N with
-             | var n => beq_string m n
-             | _     => false
-            end
-  | app M1 M2 => match N with
-              | app N1 N2 => (beq_term M1 N1) 
-                             && (beq_term M2 N2)
-              | _         => false
-              end
-  | lam x A m => match N with
-                  | lam y B n => (beq_string x y)
-                                 && (beq_type A B)
-                                 && (beq_term m n)
-                  | _ => false
-                  end
-end.
+  match M, N with
+  | var m, var n => 
+      beq_string m n
+  | app M1 M2, app N1 N2 => 
+      beq_term M1 N1 && beq_term M2 N2
+  | lam x A m, lam y B n => 
+      beq_string x y && beq_type A B && beq_term m n
+  | _,_ => false
+  end.
 
 (* Exercise 2.5 *)
 
@@ -101,14 +114,11 @@ Fixpoint typecheck (E : ctx) (t : term) : option type :=
   match t with
   | var x => E x
   | app M N => 
-    match (typecheck E M) with
-    | Some (tarr A B) => 
-      match (typecheck E N) with
-      | Some C  => if (beq_type A C) then Some B 
-                                     else None
-      | _       => None
-      end
-    | _ => None
+    match (typecheck E M), (typecheck E N) with
+    | Some (tarr A B), Some C => 
+        if beq_type A C then Some B 
+                        else None
+    | _,_ => None
     end
   | lam x A M => 
     match (typecheck (E&{x-->Some A}) M) with
@@ -129,7 +139,143 @@ nothing if there is no type).
 
 (* Exercise 2.7 *)
 
-lemma typecheck1 : typecheck empty 
+Example pos_typecheck_1 : 
+typecheck empty (lxly_x "X" "Y") = Some (X_Y_X "X" "Y").
+Proof. reflexivity. Qed.
+
+Example pos_typecheck_2 : 
+typecheck empty (lflx_ffx "X") = Some (XX_XX "X").
+Proof. reflexivity. Qed.
+
+Definition lx_xx (X: string) := 
+  lam "x" (tvar X) (app (var "x") (var "x")).
+
+Example neg_typecheck_1 : 
+typecheck empty (lx_xx "X") = None.
+Proof. reflexivity. Qed.
+
+Definition lflx_xf (X: string) :=
+  lam "f" (tarr (tvar X) (tvar X)) 
+      (lam "x" (tvar X) 
+           (app (var "x") (var "f")) ).
+
+Example neg_typecheck_2 :
+typecheck empty (lflx_xf "X") = None.
+Proof. reflexivity. Qed.
+
+(* Exercise 2.8 *)
+
+Lemma typecheck_complete : forall E t A,
+  typed E t A ->
+  typecheck E t = Some A.
+Proof.
+intros E t A H.
+induction H.
+- apply H.
+- simpl.
+  rewrite IHtyped1. rewrite IHtyped2.
+  rewrite beq_type_refl.
+  reflexivity.
+- simpl.
+  rewrite IHtyped. reflexivity.
+Qed.
+
+Ltac solve_by_inverts n :=
+  match goal with | H : ?T |- _ =>
+  match type of T with Prop =>
+    solve [
+      inversion H;
+      match n with S (S (?n')) => subst; solve_by_inverts (S n') end ]
+  end end.
+
+Ltac solve_by_invert :=
+  solve_by_inverts 1.
+
+Lemma typecheck_sound : forall E t A,
+  typecheck E t = Some A ->
+  typed E t A.
+Proof.
+intros E t.
+induction t; intros B Htc. inversion Htc.
+- apply var_typed. apply H0.
+- simpl typecheck in Htc. simpl (typecheck E t1) in Htc.
+
+unfold typecheck in Htc.
+remember (typecheck E t1) as TO1.
+  remember (typecheck E t2) as TO2.
+  destruct TO1 as [T1|].
+  + destruct T1 as [|TA TB].
+    *
+  +
+  destruct TO2 as [T2|]; try solve_by_invert.
+  destruct (beq_type T11 T2) eqn: Heqb;
+  try solve_by_invert.
+
+  apply beq_type_eq in Heqb.
+  apply app_typed; subst..
+-
+  
+
+destruct (typecheck E t1) as [T1|].
+  destruct T1 as [|TA TB].
+  + apply (Some (tvar s) = Some (tvar s)) in IHt1.
+  + destruct (typecheck E t2) as [T2|].
+  destruct (beq_type TA T2) eqn: Heqa.
+  * apply beq_type_eq in Heqa.
+    rewrite <- Heqa in IHt2.
+    {destruct (beq_type TB B) eqn: Heqb.
+    - apply beq_type_eq in Heqb.
+      rewrite Heqb in IHt1.
+      apply app_typed with (A := TA).
+      apply IHt1. reflexivity.
+      apply IHt2. reflexivity.
+    - Search solve_by_invert.
+Search "iff".
+    }
+    apply app_typed (A := TA) (B := TB).
+  *
+  assert (Some T1 = Some T1) as HtypT1.
+  reflexivity.
+  apply IHt1 in HtypT1.
+  destruct T1 as [|TA TB].
+  + admit.
+  + apply app_typed 
+    with (E := E) (M := t1) (N := t2) 
+    (A := TA) (B := B).
+    * 
+  + inversion app.
+
+Admitted.
+
+(*
+Fixpoint typecheck (E : ctx) (t : term) : option type :=
+  match t with
+  | var x => E x
+  | app M N => 
+    match (typecheck E M), (typecheck E N) with
+    | Some (tarr A B), Some C => 
+        if beq_type A C then Some B 
+                        else None
+    | _,_ => None
+    end
+  | lam x A M => 
+    match (typecheck (E&{x-->Some A}) M) with
+    | Some B => Some (tarr A B)
+    | _      => None
+    end
+  end.
+
+Inductive typed : ctx -> term -> type -> Prop :=
+  | var_typed : forall E x A, 
+    E x = Some A -> 
+    typed E (var x) A
+  | app_typed : forall E M N A B,
+    typed E M (tarr A B) ->
+    typed E N A ->
+    typed E (app M N) B
+  | lam_typed : forall E x M A B,
+    typed (E & { x --> Some A}) M B ->
+    typed E (lam x A M) (tarr A B).
 
 Inductive type :=
 | tvar : string -> type
@@ -140,6 +286,60 @@ Inductive term :=
 | app : term -> term -> term
 | lam : string -> type -> term -> term .
 
+  
+    inversion IHt1. with (A := T1).
+ try solve by inversion;
+    destruct T1 as [|T11 T12]; try solve by inversion.
 
+apply app_typed.
+eval typecheck in Htc.
+apply app_typed with (A := typecheck E t1).
+- eval typecheck in IHt1.
+
+apply app_typed with (A := . destruct typed. destruct typecheck in IHt1.
+  
+- remember (typecheck E t1) as TO1.
+  remember (typecheck E t2) as TO2.
+  destruct TO1 as [T1|]; try solve by inversion;
+  destruct T1 as [|T11 T12]; try solve by inversion.
+ destruct typecheck in IHt1. inversion IHt1.
++ inversion IHt1.
+
+-
+    
+
+
+
+-d apply H in IHt1.
+
+ induction typecheck.
+ destruct app in H. simpl H. rewrite H in IHt1.
+- apply H in IHt1. simpl typecheck in H.
+- apply app_typed.
+ast
+Lemma typecheck_sound : forall E t A,
+  typecheck E t = Some A ->
+  typed E t A.
+Proof with eauto.
+intros E t.
+induction t; intros B Htc. inversion Htc.
+- apply var_typed. apply H0.
+- remember (typecheck E t1) as TO1.
+  remember (typecheck E t2) as TO2.
+  destruct TO1 as [T1|].
+  assert (Some T1 = Some T1) as HtypT1.
+  reflexivity.
+  apply IHt1 in HtypT1.
+  destruct T1 as [|TA TB].
+  + admit.
+  + apply app_typed 
+    with (E := E) (M := t1) (N := t2) 
+    (A := TA) (B := B).
+    * 
+  + inversion app.
+
+Admitted.
+
+*)
 
 
