STLC2.v
@@ -1,0 +1,139 @@
+Require Export stlc.Maps.
+
+Inductive ty : Type := 
+  | TVar  : string -> ty 
+  | TArrow : ty -> ty -> ty.
+
+Inductive tm : Type :=
+  | tvar : string -> tm
+  | tapp : tm -> tm -> tm
+  | tabs : string -> ty -> tm -> tm.
+
+Definition context := partial_map ty.
+
+Definition extend {A:Type} (Gamma : partial_map A) (x:string) (T : A) :=
+  fun x' => if beq_string x x' then Some T else Gamma x'.
+
+Inductive has_type : context -> tm -> ty -> Prop :=
+  | T_Var : forall Gamma x T,
+      Gamma x = Some T ->
+      has_type Gamma (tvar x) T
+  | T_Abs : forall Gamma x T11 T12 t12,
+      has_type (extend Gamma x T11) t12 T12 -> 
+      has_type Gamma (tabs x T11 t12) (TArrow T11 T12)
+  | T_App : forall T11 T12 Gamma t1 t2,
+      has_type Gamma t1 (TArrow T11 T12) -> 
+      has_type Gamma t2 T11 -> 
+      has_type Gamma (tapp t1 t2) T12.
+
+Fixpoint beq_ty (T1 T2:ty) : bool :=
+  match T1,T2 with
+  | TVar a, TVar b => beq_string a b
+  | TArrow T11 T12, TArrow T21 T22 =>
+      andb (beq_ty T11 T21) (beq_ty T12 T22)
+  | _,_ => 
+      false
+  end.
+
+Lemma beq_ty_refl : forall T1,
+  beq_ty T1 T1 = true.
+Proof.
+  intros T1. induction T1; simpl.
+    apply beq_string_true_iff. reflexivity.
+    rewrite IHT1_1. rewrite IHT1_2. reflexivity.  Qed.
+
+Lemma beq_ty__eq : forall T1 T2,
+  beq_ty T1 T2 = true -> T1 = T2.
+Proof.
+  intros T1. induction T1; intros T2 Hbeq; destruct T2; inversion Hbeq.
+  - apply beq_string_true_iff in H0. rewrite H0. reflexivity.
+  - apply andb_prop in H0. inversion H0 as [Hbeq1 Hbeq2].
+    apply IHT1_1 in Hbeq1. apply IHT1_2 in Hbeq2. subst... reflexivity. Qed.
+
+Fixpoint type_check (Gamma:context) (t:tm) : option ty :=
+  match t with
+  | tvar x => Gamma x
+  | tabs x T11 t12 => match type_check (extend Gamma x T11) t12 with
+                          | Some T12 => Some (TArrow T11 T12)
+                          | _ => None
+                        end
+  | tapp t1 t2 => match type_check Gamma t1, type_check Gamma t2 with
+                      | Some (TArrow T11 T12),Some T2 =>
+                        if beq_ty T11 T2 then Some T12 else None
+                      | _,_ => None
+                    end
+  end.
+
+Ltac solve_by_inverts n :=
+  match goal with | H : ?T |- _ =>
+  match type of T with Prop =>
+    solve [
+      inversion H;
+      match n with S (S (?n')) => subst; solve_by_inverts (S n') end ]
+  end end.
+
+Ltac solve_by_invert :=
+  solve_by_inverts 1.
+
+Fixpoint subst (x:string) (s:tm) (t:tm) : tm :=
+  match t with
+  | tvar x' => 
+      if beq_string x x' then s else t
+  | tabs x' T t1 => 
+      tabs x' T (if beq_string x x' then t1 else (subst x s t1)) 
+  | tapp t1 t2 => 
+      tapp (subst x s t1) (subst x s t2)
+  end.
+
+Theorem type_checking_sound : forall Gamma t T,
+  type_check Gamma t = Some T -> has_type Gamma t T.
+Proof.
+  intros Gamma t. generalize dependent Gamma.
+  induction t; intros Gamma T Htc; inversion Htc.
+  - apply T_Var. apply H0.
+  - remember (type_check Gamma t1) as TO1.
+    remember (type_check Gamma t2) as TO2.
+    destruct TO1 as [T1|]; try solve_by_invert;
+    destruct T1 as [|T11 T12]; try solve_by_invert.
+    destruct TO2 as [T2|]; try solve_by_invert.
+    remember (beq_ty T11 T2) as b.
+    destruct b; try solve_by_invert.
+    symmetry in Heqb. apply beq_ty__eq in Heqb.
+    inversion H0; subst... 
+    apply T_App with (T11 := T2) (T12 := T).
+    symmetry in HeqTO1.
+    apply IHt1 in HeqTO1. apply HeqTO1.
+    symmetry in HeqTO2.
+    apply IHt2 in HeqTO2. apply HeqTO2.
+  - remember (extend Gamma s t) as G'.
+    remember (type_check G' t0) as TO2.
+    destruct TO2; try solve_by_invert.
+    inversion H0. apply T_Abs. rewrite <- HeqG'.
+    apply IHt. rewrite HeqTO2. reflexivity. Qed.
+
+
+Lemma typecheck_complete : forall E t A,
+  has_type E t A ->
+  type_check E t = Some A.
+Proof.
+intros E t A H.
+induction H.
+- apply H.
+- simpl.
+  rewrite IHtyped1. rewrite IHtyped2.
+  rewrite beq_ty_refl.
+  reflexivity.
+- simpl.
+  rewrite IHtyped. reflexivity.
+Qed.
+
+
+
+
+
+
+
+
+
+
+
