STLC3.v
@@ -1,0 +1,200 @@
+Require Export stlc.Maps.
+
+Inductive type : Type := 
+  | tvar  : string -> type 
+  | tarr : type -> type -> type.
+
+Inductive term : Type :=
+  | var : string -> term
+  | app : term -> term -> term
+  | lam : string -> type -> term -> term.
+
+Definition ctx := partial_map type.
+
+(* Exercise 2.1 *)
+
+Definition X_Y_X (X:string) (Y:string) : type := 
+  tarr (tvar X) (tarr (tvar Y) (tvar X)).
+
+Definition XX_XX (X:string) : type := 
+  tarr (tarr (tvar X) (tvar X)) (tarr (tvar X) (tvar X)).
+
+(* Exercise 2.2 *)
+
+Definition lxly_x (X:string) (Y:string) : term :=
+  lam "x" (tvar X) (lam "y" (tvar Y) (var "x")).
+
+Definition lflx_ffx (X:string) : term :=
+  lam "f" (tarr (tvar X) (tvar X)) 
+      (lam  "x" (tvar X) 
+            (app  (var "f") 
+                  (app  (var "f") 
+                        (var "x")))).
+
+(* Exercise 2.3 *)
+
+Inductive typed : ctx -> term -> type -> Prop :=
+  | var_typed : forall E x A,
+      E x = Some A ->
+      typed E (var x) A
+  | app_typed : forall A B E M N,
+      typed E M (tarr A B) ->
+      typed E N A -> 
+      typed E (app M N) B
+  | lam_typed : forall E x A B M,
+      typed (update E x A) M B -> 
+      typed E (lam x A M) (tarr A B).
+
+(* Exercise 2.4 *)
+
+Lemma test : typed  empty
+                    (lxly_x "X" "Y") 
+                    (X_Y_X "X" "Y").
+Proof.
+unfold lxly_x. unfold X_Y_X.
+apply lam_typed. 
+apply lam_typed. 
+apply var_typed.
+reflexivity.
+Qed.
+
+(* Exercise 2.5 *)
+
+(*  To build a typechecker, we first need to define 
+    a helper function for type equality and prove that
+    it actually defines equality. *)
+Fixpoint beq_type (A B:type) : bool :=
+  match A,B with
+  | tvar a, tvar b => beq_string a b
+  | tarr A1 A2, tarr B1 B2 =>
+      andb (beq_type A1 B1) (beq_type A2 B2)
+  | _,_ => 
+      false
+  end.
+
+Lemma beq_type_refl : forall A,
+  beq_type A A = true.
+Proof.
+  intros A1. induction A1; simpl.
+  apply beq_string_true_iff. reflexivity.
+  rewrite IHA1_1. rewrite IHA1_2. reflexivity.  Qed.
+
+Lemma beq_type_eq : forall A B,
+  beq_type A B = true -> A = B.
+Proof.
+  intros A. induction A; intros A Hbeq; destruct A; inversion Hbeq.
+  - apply beq_string_true_iff in H0. rewrite H0. reflexivity.
+  - apply andb_prop in H0. inversion H0 as [Hbeq1 Hbeq2].
+    apply IHA1 in Hbeq1. apply IHA2 in Hbeq2. subst... reflexivity. Qed.
+
+Fixpoint typecheck (E:ctx) (t:term) : option type :=
+  match t with
+  | var x     => E x
+  | app M N   => match typecheck E M, typecheck E N with
+                 | Some (tarr A B),Some A1 =>
+                    if beq_type A A1 then Some B else None
+                 | _,_ => None
+                    end
+  | lam x A M => match typecheck (update E x A) M with
+                 | Some B => Some (tarr A B)
+                 | _ => None
+                 end
+  end.
+
+(* Exercise 2.6 *)
+
+(* 
+The typing judgement [typed] will tell us for a given
+context, term and type whether the term is of that type.
+The type checker [typecheck] will tell us for a given
+context and term what the type is (or it will return
+nothing if there is no type).
+ *)
+
+(* Exercise 2.7 *)
+
+Example pos_typecheck_1 : 
+typecheck empty (lxly_x "X" "Y") = Some (X_Y_X "X" "Y").
+Proof. reflexivity. Qed.
+
+Example pos_typecheck_2 : 
+typecheck empty (lflx_ffx "X") = Some (XX_XX "X").
+Proof. reflexivity. Qed.
+
+Definition lx_xx (X: string) := 
+  lam "x" (tvar X) (app (var "x") (var "x")).
+
+Example neg_typecheck_1 : 
+typecheck empty (lx_xx "X") = None.
+Proof. reflexivity. Qed.
+
+Definition lflx_xf (X: string) :=
+  lam "f" (tarr (tvar X) (tvar X)) 
+      (lam "x" (tvar X) 
+           (app (var "x") (var "f")) ).
+
+Example neg_typecheck_2 :
+typecheck empty (lflx_xf "X") = None.
+Proof. reflexivity. Qed.
+
+(* Exercise 2.8 *)
+
+Lemma typecheck_complete : forall E t A,
+  typed E t A ->
+  typecheck E t = Some A.
+Proof.
+intros E t A H.
+induction H.
+- apply H.
+- simpl.
+  rewrite IHtyped1. rewrite IHtyped2.
+  rewrite beq_type_refl.
+  reflexivity.
+- simpl.
+  rewrite IHtyped. reflexivity.
+Qed.
+
+Ltac solve_by_invert :=
+  match goal with 
+  | H : ?T 
+  |- _ => match type of T with 
+          | Prop => solve [inversion H]
+          end
+  end.
+
+Lemma typecheck_sound : forall E t A,
+  typecheck E t = Some A -> typed E t A.
+Proof.
+  intros E t. generalize dependent E.
+  induction t; intros E T Htc; inversion Htc.
+  - apply var_typed. apply H0.
+  - remember (typecheck E t1) as TO1.
+    remember (typecheck E t2) as TO2.
+    destruct TO1 as [A|]; try solve_by_invert;
+    destruct A as [|A1 A2]; try solve_by_invert.
+    destruct TO2 as [B|]; try solve_by_invert.
+    remember (beq_type A1 B) as b.
+    destruct b; try solve_by_invert.
+    symmetry in Heqb. apply beq_type_eq in Heqb.
+    inversion H0; subst... 
+    apply app_typed with (A := B) (B := T).
+    symmetry in HeqTO1.
+    apply IHt1 in HeqTO1. apply HeqTO1.
+    symmetry in HeqTO2.
+    apply IHt2 in HeqTO2. apply HeqTO2.
+  - remember (update E s t) as G'.
+    remember (typecheck G' t0) as TO2.
+    destruct TO2; try solve_by_invert.
+    inversion H0. apply lam_typed. rewrite <- HeqG'.
+    apply IHt. rewrite HeqTO2. reflexivity. Qed.
+
+
+
+
+
+
+
+
+
+
+
